@prefix mbz: <http://purl.org/ontology/mbz#>.
@prefix owl: <http://www.w3.org/2002/07/owl#>.
@prefix mo: <http://purl.org/ontology/mo/>.
@prefix rdfs: <http://www.w3.org/2000/01/rdf-schema#>.
@prefix frbr: <http://purl.org/vocab/frbr/core#>.

mbz:version 
	a owl:ObjectProperty;
	rdfs:label "cover and version";
	rdfs:comment "covers or other versions";
	rdfs:domain mo:Release;
	rdfs:range mo:Release;
	rdfs:subPropertyOf frbr:relatedEndeavour;
	.

mbz:altered_version
	a owl:ObjectProperty;
	rdfs:label "altered versions";
	rdfs:comment "altered version in a creative way (remixes etc.)";
	rdfs:domain mo:Record;
	rdfs:range mo:Record;
	rdfs:subPropertyOf frbr:relatedEndeavour;
	.

mbz:first_release
	a owl:ObjectProperty;
	rdfs:label "first release";
	rdfs:comment """
Indicates that the two albums contain mostly the same audio material. 
This means that the audio data is *exactly* identical. 
No remastering has been applied, but it is okay if bonus 
tracks were added or the order of the tracks was 
changed. Please take care to always point to 
the *first* version ever released! 
See http://wiki.musicbrainz.org/EarliestReleaseRelationshipType
""";
	rdfs:domain mo:Release;
	rdfs:range mo:Release;
	rdfs:subPropertyOf mbz:version;
	.

mbz:remaster
	a owl:ObjectProperty;
	rdfs:label "remaster";
	rdfs:comment """
Indicates that an album is a remaster of another album. 
This means that the audio data was changed in this process 
but the same original recording material was used. 
Please take care to always point to the *first* version ever released!
See http://wiki.musicbrainz.org/RemasterRelationshipType
""";
	rdfs:domain mo:Release;
	rdfs:range mo:Release;
	rdfs:subPropertyOf mbz:version;
	.

mbz:remix
	a owl:ObjectProperty;
	rdfs:label "remaster";
	rdfs:comment """
Indicates that an album includes remixed versions of all (or most of) the tracks of the other album.
See http://wiki.musicbrainz.org/RemixRelationshipType
""";
	rdfs:domain mo:Record;
	rdfs:range mo:Record;
	rdfs:subPropertyOf mbz:altered_version;
	.

mbz:mashup
	a owl:ObjectProperty;
	rdfs:label "mashes up";
	rdfs:comment """
Indicates that albums were mashed up on this album. 
This means that two pieces of music by different artists 
are mixed together, over each other, or otherwise 
combined into a single work (usually by a third artist, the remixer).
""";
	rdfs:domain mo:Record;
	rdfs:range mo:Record;
	rdfs:subPropertyOf mbz:altered_version;
	.

mbz:dj-mix
	a owl:ObjectProperty;
	rdfs:label "DJ mix";
	rdfs:comment """
Indicates that all (or most of) the tracks of an album 
were mixed together from all (or most of) the tracks 
from another album to form a so called DJ-Mix. The tracks 
might have been altered by pitching (so that the tempo 
of one track matches the tempo of the following track) 
and fading (so that one track blends in smoothly with 
the other). If the tracks have been more substantially 
altered, the remix relationship type is more appropriate.
See http://wiki.musicbrainz.org/DJMixRelationshipType
""";
	rdfs:domain mo:Record;
	rdfs:range mo:Record;
	# In the DB schema, it is is the subproperty of "compilations" (???)
	rdfs:subPropertyOf mbz:altered_version;
	.

mbz:live
	a owl:ObjectProperty;
	rdfs:label "live performance";
	rdfs:comment """
Indicates that an album was performed live and 
released as another album. Please use this relationship 
only if (almost) every track of the original recording 
was performed on the live version, not for normal live recordings.
""";
	rdfs:domain mo:Record;
	rdfs:range mo:Record;
	rdfs:subPropertyOf mbz:version;
	.

mbz:cover
	a owl:ObjectProperty;
	rdfs:label "cover";
	rdfs:comment """
Indicates a cover version of a album. This means that 
another artist performed the same songs. Please take 
care to always point to the *first* version ever released!
See http://wiki.musicbrainz.org/CoverRelationshipType
""";
	rdfs:domain mo:Record;
	rdfs:range mo:Record;
	rdfs:subPropertyOf mbz:version;
	.

mbz:translation
	a owl:ObjectProperty;
	rdfs:label "translation";
	rdfs:comment """
Indicates that an album has translated or transliterated 
titles on another album release. This relationship does 
not indicate a cover where the lyrics have been translated 
(that should be indicated with 'cover' instead, although both 
relationships could apply in some cases). This relationship 
should only be used when the number, order, and audio of the 
tracks on the two albums are identical, and each of the 
titles corresponds in meaning.
""";
	rdfs:domain mo:Release;
	rdfs:range mo:Release;
	rdfs:subPropertyOf mbz:version;
	.

mbz:remixer
	a owl:ObjectProperty;
	rdfs:label "remixer";
	rdfs:comment """
Indicates the person who remixed the album by taking tracks, 
substanially altering them and mixing them together with other 
material. Note that this one is used for the artist who created 
a mash-up or used samples as well.
See http://wiki.musicbrainz.org/RemixerRelationshipType
""";
	rdfs:domain mo:Record;
	rdfs:range mo:Record;
	.
